compiler/src/Compiler/Driver/CompEval.v
@@ -129,10 +129,10 @@ Section CompEval.
     Definition eval_imp_qcert (q:imp_qcert) (cenv: bindings) : option data :=
       ImpQcertEval.imp_qcert_eval_top h cenv q.
 
-    (* Language: imp_json *)
+    (* Language: imp_ejson *)
     (* XXX Is this really what we want to wrap/unwrap in data? *)
-    Definition eval_imp_json (q:imp_json) (cenv: bindings) : option data :=
-      ImpJsonEval.imp_json_eval_top_alt cenv q.
+    Definition eval_imp_ejson (q:imp_ejson) (cenv: bindings) : option data :=
+      ImpEJsonEval.imp_ejson_eval_top cenv q.
 
     (* Language: nnrcmr *)
     Definition eval_nnrcmr (q:nnrcmr) (dcenv: dbindings) : option data :=
@@ -186,7 +186,7 @@ Section CompEval.
       | Q_nnrs q => lift_output (eval_nnrs q (lift_input ev_in))
       | Q_nnrs_imp q => lift_output (eval_nnrs_imp q (lift_input ev_in))
       | Q_imp_qcert q => lift_output (eval_imp_qcert q (lift_input ev_in))
-      | Q_imp_json q => lift_output (eval_imp_json q (lift_input ev_in))
+      | Q_imp_ejson q => lift_output (eval_imp_ejson q (lift_input ev_in))
       | Q_nnrcmr q => lift_output (eval_nnrcmr q ev_in) (* XXX Does not localize, keeps distributed information XXX *)
       | Q_dnnrc q => lift_output (eval_dnnrc q ev_in) (* XXX Does not localize, keeps distributed information XXX *)
       | Q_dnnrc_typed q => lift_output (eval_dnnrc_typed q ev_in) (* XXX Does not localize, keeps distributed information XXX *)
@@ -216,7 +216,7 @@ Section CompEval.
       | Q_nnrs _ => Ev_out_unsupported ("No debug evaluation support for "++(name_of_language (language_of_query q)))
       | Q_nnrs_imp _ => Ev_out_unsupported ("No debug evaluation support for "++(name_of_language (language_of_query q)))
       | Q_imp_qcert _ => Ev_out_unsupported ("No debug evaluation support for "++(name_of_language (language_of_query q)))
-      | Q_imp_json _ => Ev_out_unsupported ("No debug evaluation support for "++(name_of_language (language_of_query q)))
+      | Q_imp_ejson _ => Ev_out_unsupported ("No debug evaluation support for "++(name_of_language (language_of_query q)))
       | Q_nnrcmr _ => Ev_out_unsupported ("No debug evaluation support for "++(name_of_language (language_of_query q)))
       | Q_dnnrc _ => Ev_out_unsupported ("No debug evaluation support for "++(name_of_language (language_of_query q)))
       | Q_dnnrc_typed _ => Ev_out_unsupported ("No debug evaluation support for "++(name_of_language (language_of_query q)))
