compiler/src/Translation/ImpQcerttoImpEJson.v
@@ -23,12 +23,12 @@ Require Import CommonRuntime.
 Require Import Imp.
 Require Import ImpQcert.
 Require Import ImpQcertEval.
-Require Import ImpJson.
-Require Import ImpJsonEval.
+Require Import ImpEJson.
+Require Import ImpEJsonEval.
 Require Import JsAst.JsNumber.
 Require Import Fresh.
 
-Section ImpJsontoJavaScriptAst.
+Section ImpQcerttoImpEJson.
   Import ListNotations.
 
   (** Translation *)
@@ -38,22 +38,22 @@ Section ImpJsontoJavaScriptAst.
 
   Context (h:brand_relation_t). (* We need a brand relation for the Q*cert side *)
 
-(*Definition mk_imp_json_expr_error msg : imp_json_expr :=
+(*Definition mk_imp_ejson_expr_error msg : imp_ejson_expr :=
     ImpExprConst (jstring msg). *)
-  Definition mk_imp_ejson_expr_error msg : imp_json_expr :=
+  Definition mk_imp_ejson_expr_error msg : imp_ejson_expr :=
     ImpExprError msg. (* XXX Error should eval to None if we want to prove stuffs! *)
-  Definition mk_imp_ejson_op op el : imp_json_expr := ImpExprOp op el.
-  Definition mk_imp_ejson_runtime_call op el : imp_json_expr := ImpExprRuntimeCall op el.
+  Definition mk_imp_ejson_op op el : imp_ejson_expr := ImpExprOp op el.
+  Definition mk_imp_ejson_runtime_call op el : imp_ejson_expr := ImpExprRuntimeCall op el.
 
-  Definition mk_string s : imp_json_expr := ImpExprConst (ejstring s).
-  Definition mk_string_array sl : imp_json_expr := ImpExprConst (ejarray (map ejstring sl)).
-  Definition mk_bag el : imp_json_expr := mk_imp_ejson_op EJSONOpArray el.
-  Definition mk_left e : imp_json_expr :=
-    mk_imp_ejson_op (EJSONOpObject ["$left"%string]) [ e ].
-  Definition mk_right e : imp_json_expr :=
-    mk_imp_ejson_op (EJSONOpObject ["$right"%string]) [ e ].
+  Definition mk_string s : imp_ejson_expr := ImpExprConst (ejstring s).
+  Definition mk_string_array sl : imp_ejson_expr := ImpExprConst (ejarray (map ejstring sl)).
+  Definition mk_bag el : imp_ejson_expr := mk_imp_ejson_op EJsonOpArray el.
+  Definition mk_left e : imp_ejson_expr :=
+    mk_imp_ejson_op (EJsonOpObject ["$left"%string]) [ e ].
+  Definition mk_right e : imp_ejson_expr :=
+    mk_imp_ejson_op (EJsonOpObject ["$right"%string]) [ e ].
 
-  Definition sortCriteria_to_json_expr (sc: string * SortDesc) : imp_json_expr :=
+  Definition sortCriteria_to_ejson_expr (sc: string * SortDesc) : imp_ejson_expr :=
     let (lbl, c) := sc in
     let o :=
         match c with
@@ -63,33 +63,33 @@ Section ImpJsontoJavaScriptAst.
     in
     ImpExprConst o.
 
-  Definition brands_to_json_expr sl : imp_json_expr :=
+  Definition brands_to_ejson_expr sl : imp_ejson_expr :=
     let j := ejarray ((List.map (fun s => ejstring s)) sl) in
     ImpExprConst j.
 
-  Definition imp_qcert_unary_op_to_imp_json (op:unary_op) el : imp_json_expr :=
+  Definition imp_qcert_unary_op_to_imp_ejson (op:unary_op) el : imp_ejson_expr :=
     match el with
     | [e] =>
       match op with
       | OpIdentity => e
-      | OpNeg => mk_imp_ejson_op EJSONOpNot [e]
-      | OpRec s => mk_imp_ejson_op (EJSONOpObject [json_key_encode s]) [e]
-      | OpDot s => mk_imp_ejson_runtime_call JSONRuntimeDeref [e; ImpExprConst (ejstring (json_key_encode s))]
-      | OpRecRemove s => mk_imp_ejson_runtime_call JSONRuntimeRemove [e; mk_string (json_key_encode s)]
+      | OpNeg => mk_imp_ejson_op EJsonOpNot [e]
+      | OpRec s => mk_imp_ejson_op (EJsonOpObject [json_key_encode s]) [e]
+      | OpDot s => mk_imp_ejson_runtime_call EJsonRuntimeDeref [e; ImpExprConst (ejstring (json_key_encode s))]
+      | OpRecRemove s => mk_imp_ejson_runtime_call EJsonRuntimeRemove [e; mk_string (json_key_encode s)]
       | OpRecProject fl =>
         mk_imp_ejson_runtime_call
-          JSONRuntimeProject ([e] ++ [mk_string_array fl])
+          EJsonRuntimeProject ([e] ++ [mk_string_array fl])
       | OpBag => mk_bag el
-      | OpSingleton => mk_imp_ejson_runtime_call JSONRuntimeSingleton el
-      | OpFlatten => mk_imp_ejson_runtime_call JSONRuntimeFlatten el
-      | OpDistinct => mk_imp_ejson_runtime_call JSONRuntimeDistinct el
+      | OpSingleton => mk_imp_ejson_runtime_call EJsonRuntimeSingleton el
+      | OpFlatten => mk_imp_ejson_runtime_call EJsonRuntimeFlatten el
+      | OpDistinct => mk_imp_ejson_runtime_call EJsonRuntimeDistinct el
       | OpOrderBy scl =>
         mk_imp_ejson_runtime_call
-          JSONRuntimeSort (e :: (List.map sortCriteria_to_json_expr scl))
-      | OpCount => mk_imp_ejson_runtime_call JSONRuntimeCount el
-      | OpToString => mk_imp_ejson_op EJSONOpToString el
-      | OpToText => mk_imp_ejson_runtime_call JSONRuntimeToText el
-      | OpLength => mk_imp_ejson_runtime_call JSONRuntimeLength el
+          EJsonRuntimeSort (e :: (List.map sortCriteria_to_ejson_expr scl))
+      | OpCount => mk_imp_ejson_runtime_call EJsonRuntimeCount el
+      | OpToString => mk_imp_ejson_op EJsonOpToString el
+      | OpToText => mk_imp_ejson_runtime_call EJsonRuntimeToText el
+      | OpLength => mk_imp_ejson_runtime_call EJsonRuntimeLength el
       | OpSubstring start len => (* XXX Should be split into two different functions *)
         let start := ImpExprConst (ejnumber (float_of_int start)) in
         let args :=
@@ -100,133 +100,133 @@ Section ImpJsontoJavaScriptAst.
               [ e; start; len ]
             end
         in
-        mk_imp_ejson_runtime_call JSONRuntimeSubstring args
+        mk_imp_ejson_runtime_call EJsonRuntimeSubstring args
       | OpLike pat oescape =>
-        mk_imp_ejson_expr_error "XXX TODO: ImpQcerttoImpJson: OpLike XXX"
+        mk_imp_ejson_expr_error "XXX TODO: ImpQcerttoImpEJson: OpLike XXX"
       | OpLeft => mk_left e
       | OpRight => mk_right e
       | OpBrand b =>
-        mk_imp_ejson_runtime_call JSONRuntimeBrand [ brands_to_json_expr (canon_brands h b); e ]
-      | OpUnbrand => mk_imp_ejson_runtime_call JSONRuntimeUnbrand el
+        mk_imp_ejson_runtime_call EJsonRuntimeBrand [ brands_to_ejson_expr (canon_brands h b); e ]
+      | OpUnbrand => mk_imp_ejson_runtime_call EJsonRuntimeUnbrand el
       | OpCast b =>
-        mk_imp_ejson_runtime_call JSONRuntimeCast [ brands_to_json_expr b; e ]
+        mk_imp_ejson_runtime_call EJsonRuntimeCast [ brands_to_ejson_expr b; e ]
       | OpNatUnary u =>
         let op :=
             match u with
-            | NatAbs => JSONRuntimeNatAbs
-            | NatLog2 => JSONRuntimeNatLog2
-            | NatSqrt => JSONRuntimeNatSqrt
+            | NatAbs => EJsonRuntimeNatAbs
+            | NatLog2 => EJsonRuntimeNatLog2
+            | NatSqrt => EJsonRuntimeNatSqrt
             end
         in
         mk_imp_ejson_runtime_call op [ e ]
-      | OpNatSum => mk_imp_ejson_runtime_call JSONRuntimeNatSum el
-      | OpNatMin => mk_imp_ejson_runtime_call JSONRuntimeNatMin el
-      | OpNatMax => mk_imp_ejson_runtime_call JSONRuntimeNatMax el
-      | OpNatMean => mk_imp_ejson_runtime_call JSONRuntimeNatArithMean el
-      | OpFloatOfNat => mk_imp_ejson_runtime_call JSONRuntimeFloatOfNat el
+      | OpNatSum => mk_imp_ejson_runtime_call EJsonRuntimeNatSum el
+      | OpNatMin => mk_imp_ejson_runtime_call EJsonRuntimeNatMin el
+      | OpNatMax => mk_imp_ejson_runtime_call EJsonRuntimeNatMax el
+      | OpNatMean => mk_imp_ejson_runtime_call EJsonRuntimeNatArithMean el
+      | OpFloatOfNat => mk_imp_ejson_runtime_call EJsonRuntimeFloatOfNat el
       | OpFloatUnary u =>
         match u with
-        | FloatNeg => mk_imp_ejson_op EJSONOpNeg [ e ]
-        | FloatSqrt => mk_imp_ejson_op EJSONOpMathSqrt [ e ]
-        | FloatExp => mk_imp_ejson_op EJSONOpMathExp [ e ]
-        | FloatLog => mk_imp_ejson_op EJSONOpMathLog [ e ]
-        | FloatLog10 => mk_imp_ejson_op EJSONOpMathLog10 [ e ]
-        | FloatCeil => mk_imp_ejson_op EJSONOpMathCeil [ e ]
-        | FloatFloor => mk_imp_ejson_op EJSONOpMathFloor [ e ]
-        | FloatAbs => mk_imp_ejson_op EJSONOpMathAbs [ e ]
+        | FloatNeg => mk_imp_ejson_op EJsonOpNeg [ e ]
+        | FloatSqrt => mk_imp_ejson_op EJsonOpMathSqrt [ e ]
+        | FloatExp => mk_imp_ejson_op EJsonOpMathExp [ e ]
+        | FloatLog => mk_imp_ejson_op EJsonOpMathLog [ e ]
+        | FloatLog10 => mk_imp_ejson_op EJsonOpMathLog10 [ e ]
+        | FloatCeil => mk_imp_ejson_op EJsonOpMathCeil [ e ]
+        | FloatFloor => mk_imp_ejson_op EJsonOpMathFloor [ e ]
+        | FloatAbs => mk_imp_ejson_op EJsonOpMathAbs [ e ]
         end
-      | OpFloatTruncate => mk_imp_ejson_op EJSONOpMathTrunc [e]
-      | OpFloatSum => mk_imp_ejson_runtime_call JSONRuntimeSum el
-      | OpFloatMean => mk_imp_ejson_runtime_call JSONRuntimeArithMean el
-      | OpFloatBagMin => mk_imp_ejson_op EJSONOpMathMinApply [e]
-      | OpFloatBagMax => mk_imp_ejson_op EJSONOpMathMaxApply [e]
+      | OpFloatTruncate => mk_imp_ejson_op EJsonOpMathTrunc [e]
+      | OpFloatSum => mk_imp_ejson_runtime_call EJsonRuntimeSum el
+      | OpFloatMean => mk_imp_ejson_runtime_call EJsonRuntimeArithMean el
+      | OpFloatBagMin => mk_imp_ejson_op EJsonOpMathMinApply [e]
+      | OpFloatBagMax => mk_imp_ejson_op EJsonOpMathMaxApply [e]
       | OpForeignUnary fu =>
-        mk_imp_ejson_expr_error "XXX TODO: ImpQcerttoImpJson.imp_qcert_unary_op_to_imp_json OpForeignUnary"
+        mk_imp_ejson_expr_error "XXX TODO: ImpQcerttoImpEJson.imp_qcert_unary_op_to_imp_ejson OpForeignUnary"
       end
     | _ => mk_imp_ejson_expr_error "wrong number of arguments"
     end.
 
-  Definition imp_qcert_binary_op_to_imp_json (op:binary_op) el : imp_json_expr :=
+  Definition imp_qcert_binary_op_to_imp_ejson (op:binary_op) el : imp_ejson_expr :=
     match el with
     | [e1; e2] =>
       match op with
-      | OpEqual => mk_imp_ejson_runtime_call JSONRuntimeEqual el
-      | OpRecConcat => mk_imp_ejson_runtime_call JSONRuntimeRecConcat el
-      | OpRecMerge => mk_imp_ejson_runtime_call JSONRuntimeRecMerge el
-      | OpAnd => mk_imp_ejson_op EJSONOpAnd el
-      | OpOr => mk_imp_ejson_op EJSONOpOr el
+      | OpEqual => mk_imp_ejson_runtime_call EJsonRuntimeEqual el
+      | OpRecConcat => mk_imp_ejson_runtime_call EJsonRuntimeRecConcat el
+      | OpRecMerge => mk_imp_ejson_runtime_call EJsonRuntimeRecMerge el
+      | OpAnd => mk_imp_ejson_op EJsonOpAnd el
+      | OpOr => mk_imp_ejson_op EJsonOpOr el
       | OpLt =>
-        mk_imp_ejson_op EJSONOpLt
-                       [ mk_imp_ejson_runtime_call JSONRuntimeCompare [e1; e2];
+        mk_imp_ejson_op EJsonOpLt
+                       [ mk_imp_ejson_runtime_call EJsonRuntimeCompare [e1; e2];
                          ImpExprConst (ejnumber zero) ]
       | OpLe =>
-        mk_imp_ejson_op EJSONOpLe
-                       [ mk_imp_ejson_runtime_call JSONRuntimeCompare [e1; e2];
+        mk_imp_ejson_op EJsonOpLe
+                       [ mk_imp_ejson_runtime_call EJsonRuntimeCompare [e1; e2];
                          ImpExprConst (ejnumber zero) ]
-      | OpBagUnion => mk_imp_ejson_runtime_call JSONRuntimeBunion [e1; e2]
-      | OpBagDiff => mk_imp_ejson_runtime_call JSONRuntimeBminus [e1; e2]
-      | OpBagMin => mk_imp_ejson_runtime_call JSONRuntimeBmin [e1; e2]
-      | OpBagMax => mk_imp_ejson_runtime_call JSONRuntimeBmax [e1; e2]
-      | OpBagNth => mk_imp_ejson_runtime_call JSONRuntimeBnth [e1; e2]
-      | OpContains => mk_imp_ejson_runtime_call JSONRuntimeContains [e1; e2]
-      | OpStringConcat => mk_imp_ejson_op EJSONOpAddString el
-      | OpStringJoin => mk_imp_ejson_runtime_call JSONRuntimeStringJoin [e1; e2]
+      | OpBagUnion => mk_imp_ejson_runtime_call EJsonRuntimeBunion [e1; e2]
+      | OpBagDiff => mk_imp_ejson_runtime_call EJsonRuntimeBminus [e1; e2]
+      | OpBagMin => mk_imp_ejson_runtime_call EJsonRuntimeBmin [e1; e2]
+      | OpBagMax => mk_imp_ejson_runtime_call EJsonRuntimeBmax [e1; e2]
+      | OpBagNth => mk_imp_ejson_runtime_call EJsonRuntimeBnth [e1; e2]
+      | OpContains => mk_imp_ejson_runtime_call EJsonRuntimeContains [e1; e2]
+      | OpStringConcat => mk_imp_ejson_op EJsonOpAddString el
+      | OpStringJoin => mk_imp_ejson_runtime_call EJsonRuntimeStringJoin [e1; e2]
       | OpNatBinary opa =>
         match opa with
-        | NatPlus => mk_imp_ejson_runtime_call JSONRuntimeNatPlus [e1; e2]
-        | NatMinus => mk_imp_ejson_runtime_call JSONRuntimeNatMinus [e1; e2]
-        | NatMult => mk_imp_ejson_runtime_call JSONRuntimeNatMult [e1; e2]
-        | NatDiv => mk_imp_ejson_runtime_call JSONRuntimeNatDiv [e1; e2]
-        | NatRem => mk_imp_ejson_runtime_call JSONRuntimeNatRem [e1; e2]
-        | NatMin => mk_imp_ejson_runtime_call JSONRuntimeNatMin [e1; e2]
-        | NatMax => mk_imp_ejson_runtime_call JSONRuntimeNatMax [e1; e2]
+        | NatPlus => mk_imp_ejson_runtime_call EJsonRuntimeNatPlus [e1; e2]
+        | NatMinus => mk_imp_ejson_runtime_call EJsonRuntimeNatMinus [e1; e2]
+        | NatMult => mk_imp_ejson_runtime_call EJsonRuntimeNatMult [e1; e2]
+        | NatDiv => mk_imp_ejson_runtime_call EJsonRuntimeNatDiv [e1; e2]
+        | NatRem => mk_imp_ejson_runtime_call EJsonRuntimeNatRem [e1; e2]
+        | NatMin => mk_imp_ejson_runtime_call EJsonRuntimeNatMin [e1; e2]
+        | NatMax => mk_imp_ejson_runtime_call EJsonRuntimeNatMax [e1; e2]
         end
       | OpFloatBinary opa =>
         match opa with
-        | FloatPlus => mk_imp_ejson_op EJSONOpAddNumber [e1; e2]
-        | FloatMinus => mk_imp_ejson_op EJSONOpSub [e1; e2]
-        | FloatMult => mk_imp_ejson_op EJSONOpMult [e1; e2]
-        | FloatDiv => mk_imp_ejson_op EJSONOpDiv [e1; e2]
-        | FloatPow => mk_imp_ejson_op EJSONOpMathPow [e1; e2]
-        | FloatMin => mk_imp_ejson_op EJSONOpMathMin [e1; e2]
-        | FloatMax => mk_imp_ejson_op EJSONOpMathMax [e1; e2]
+        | FloatPlus => mk_imp_ejson_op EJsonOpAddNumber [e1; e2]
+        | FloatMinus => mk_imp_ejson_op EJsonOpSub [e1; e2]
+        | FloatMult => mk_imp_ejson_op EJsonOpMult [e1; e2]
+        | FloatDiv => mk_imp_ejson_op EJsonOpDiv [e1; e2]
+        | FloatPow => mk_imp_ejson_op EJsonOpMathPow [e1; e2]
+        | FloatMin => mk_imp_ejson_op EJsonOpMathMin [e1; e2]
+        | FloatMax => mk_imp_ejson_op EJsonOpMathMax [e1; e2]
         end
       | OpFloatCompare opa =>
         match opa with
-        | FloatLt => mk_imp_ejson_op EJSONOpLt [e1; e2]
-        | FloatLe => mk_imp_ejson_op EJSONOpLe [e1; e2]
-        | FloatGt => mk_imp_ejson_op EJSONOpGt [e1; e2]
-        | FloatGe => mk_imp_ejson_op EJSONOpGe [e1; e2]
+        | FloatLt => mk_imp_ejson_op EJsonOpLt [e1; e2]
+        | FloatLe => mk_imp_ejson_op EJsonOpLe [e1; e2]
+        | FloatGt => mk_imp_ejson_op EJsonOpGt [e1; e2]
+        | FloatGe => mk_imp_ejson_op EJsonOpGe [e1; e2]
         end
       | OpForeignBinary fb =>
       (* foreign_to_ajavascript_binary_op fb [e1; e2] *)
-        mk_imp_ejson_expr_error "XXX TODO: ImpQcerttoImpJson.imp_qcert_binary_op_to_imp_json(OpForeignBinary): not yet implemented XXX" (* XXX TODO  *)
+        mk_imp_ejson_expr_error "XXX TODO: ImpQcerttoImpEJson.imp_qcert_binary_op_to_imp_ejson(OpForeignBinary): not yet implemented XXX" (* XXX TODO  *)
       end
-    | _ => mk_imp_ejson_expr_error "imp_qcert_binary_op_to_imp_json: wrong number of arguments"
+    | _ => mk_imp_ejson_expr_error "imp_qcert_binary_op_to_imp_ejson: wrong number of arguments"
     end.
 
-  Definition imp_qcert_op_to_imp_json (op:imp_qcert_op) el : imp_json_expr :=
+  Definition imp_qcert_op_to_imp_ejson (op:imp_qcert_op) el : imp_ejson_expr :=
     match op with
-    | QcertOpUnary op => imp_qcert_unary_op_to_imp_json op el
-    | QcertOpBinary op => imp_qcert_binary_op_to_imp_json op el
+    | QcertOpUnary op => imp_qcert_unary_op_to_imp_ejson op el
+    | QcertOpBinary op => imp_qcert_binary_op_to_imp_ejson op el
     end.
 
-  Definition mk_either_expr (el:list imp_json_expr) : imp_json_expr :=
-    mk_imp_ejson_runtime_call JSONRuntimeEither el.
+  Definition mk_either_expr (el:list imp_ejson_expr) : imp_ejson_expr :=
+    mk_imp_ejson_runtime_call EJsonRuntimeEither el.
 
-  Definition mk_to_left_expr (el:list imp_json_expr) : imp_json_expr :=
-    mk_imp_ejson_runtime_call JSONRuntimeToLeft el.
+  Definition mk_to_left_expr (el:list imp_ejson_expr) : imp_ejson_expr :=
+    mk_imp_ejson_runtime_call EJsonRuntimeToLeft el.
 
-  Definition mk_to_right_expr (el:list imp_json_expr) : imp_json_expr :=
-    mk_imp_ejson_runtime_call JSONRuntimeToRight el.
+  Definition mk_to_right_expr (el:list imp_ejson_expr) : imp_ejson_expr :=
+    mk_imp_ejson_runtime_call EJsonRuntimeToRight el.
 
-  Definition imp_qcert_runtime_call_to_imp_json
+  Definition imp_qcert_runtime_call_to_imp_ejson
              (op:imp_qcert_runtime_op)
-             (el:list imp_json_expr) : imp_json_expr :=
+             (el:list imp_ejson_expr) : imp_ejson_expr :=
     match op with
     | QcertRuntimeGroupby s ls =>
       mk_imp_ejson_runtime_call
-        JSONRuntimeGroupBy
+        EJsonRuntimeGroupBy
         ((ImpExprConst (ejstring s))
            :: (ImpExprConst (ejarray (map ejstring ls)))
            :: el)
@@ -234,30 +234,30 @@ Section ImpJsontoJavaScriptAst.
     | QcertRuntimeToLeft => mk_to_left_expr el
     | QcertRuntimeToRight => mk_to_right_expr el
     | QcertRuntimeDeref =>
-      mk_imp_ejson_runtime_call JSONRuntimeDeref el (* XXX ???? TODO *)
+      mk_imp_ejson_runtime_call EJsonRuntimeDeref el (* XXX ???? TODO *)
     end.
 
-  Fixpoint imp_qcert_expr_to_imp_json (exp: imp_qcert_expr) : imp_json_expr :=
+  Fixpoint imp_qcert_expr_to_imp_ejson (exp: imp_qcert_expr) : imp_ejson_expr :=
     match exp with
     | ImpExprError msg => ImpExprError msg
     | ImpExprVar v => ImpExprVar v
     | ImpExprConst d => ImpExprConst (@data_to_ejson _ _ _ (normalize_data h d)) (* XXX Add normalization *)
-    | ImpExprOp op el => imp_qcert_op_to_imp_json op (map imp_qcert_expr_to_imp_json el)
-    | ImpExprRuntimeCall op el => imp_qcert_runtime_call_to_imp_json op (map imp_qcert_expr_to_imp_json el)
+    | ImpExprOp op el => imp_qcert_op_to_imp_ejson op (map imp_qcert_expr_to_imp_ejson el)
+    | ImpExprRuntimeCall op el => imp_qcert_runtime_call_to_imp_ejson op (map imp_qcert_expr_to_imp_ejson el)
     end.
 
-  Fixpoint imp_qcert_stmt_to_imp_json (avoid: list string) (stmt: imp_qcert_stmt): imp_json_stmt :=
+  Fixpoint imp_qcert_stmt_to_imp_ejson (avoid: list string) (stmt: imp_qcert_stmt): imp_ejson_stmt :=
     match stmt with
     | ImpStmtBlock lv ls =>
       ImpStmtBlock
         (map (fun xy => (fst xy,
-                         lift imp_qcert_expr_to_imp_json (snd xy))) lv)
-        (map (imp_qcert_stmt_to_imp_json ((List.map fst lv) ++ avoid)) ls)
+                         lift imp_qcert_expr_to_imp_ejson (snd xy))) lv)
+        (map (imp_qcert_stmt_to_imp_ejson ((List.map fst lv) ++ avoid)) ls)
     | ImpStmtAssign v e =>
-      ImpStmtAssign v (imp_qcert_expr_to_imp_json e)
+      ImpStmtAssign v (imp_qcert_expr_to_imp_ejson e)
     | ImpStmtFor v e s =>
       let avoid := v :: avoid in
-      let e := imp_qcert_expr_to_imp_json e in
+      let e := imp_qcert_expr_to_imp_ejson e in
       let src_id := fresh_var "src" avoid in
       let avoid := src_id :: avoid in
       let i_id := fresh_var "i" avoid in
@@ -267,34 +267,34 @@ Section ImpJsontoJavaScriptAst.
       ImpStmtBlock
         [ (src_id, Some e) ]
         [ ImpStmtForRange
-            i_id (ImpExprConst (ejnumber zero)) (ImpExprOp EJSONOpArrayLength [ src ])
+            i_id (ImpExprConst (ejnumber zero)) (ImpExprOp EJsonOpArrayLength [ src ])
             (ImpStmtBlock
-               [ (v, Some (ImpExprOp EJSONOpArrayAccess [ src; i ])) ]
-               [ imp_qcert_stmt_to_imp_json avoid s ]) ]
+               [ (v, Some (ImpExprOp EJsonOpArrayAccess [ src; i ])) ]
+               [ imp_qcert_stmt_to_imp_ejson avoid s ]) ]
     | ImpStmtForRange v e1 e2 s =>
       ImpStmtForRange v
-                      (imp_qcert_expr_to_imp_json e1)
-                      (imp_qcert_expr_to_imp_json e2)
-                      (imp_qcert_stmt_to_imp_json (v :: avoid) s)
+                      (imp_qcert_expr_to_imp_ejson e1)
+                      (imp_qcert_expr_to_imp_ejson e2)
+                      (imp_qcert_stmt_to_imp_ejson (v :: avoid) s)
     | ImpStmtIf e s1 s2 =>
-      ImpStmtIf (imp_qcert_expr_to_imp_json e)
-                (imp_qcert_stmt_to_imp_json avoid s1)
-                (imp_qcert_stmt_to_imp_json avoid s2)
+      ImpStmtIf (imp_qcert_expr_to_imp_ejson e)
+                (imp_qcert_stmt_to_imp_ejson avoid s1)
+                (imp_qcert_stmt_to_imp_ejson avoid s2)
     end.
 
 
-  Definition imp_qcert_function_to_imp_json (f:imp_qcert_function) : imp_json_function :=
+  Definition imp_qcert_function_to_imp_ejson (f:imp_qcert_function) : imp_ejson_function :=
     match f with
-    | ImpFun v s ret => ImpFun v (imp_qcert_stmt_to_imp_json [v] s) ret
+    | ImpFun v s ret => ImpFun v (imp_qcert_stmt_to_imp_ejson [v] s) ret
     end.
 
-  Fixpoint imp_qcert_to_imp_json (i:imp_qcert) : imp_json :=
+  Fixpoint imp_qcert_to_imp_ejson (i:imp_qcert) : imp_ejson :=
     match i with
     | ImpLib l =>
       ImpLib
         (List.map
            (fun (decl: string * imp_qcert_function) =>
-              let (name, def) := decl in (name, imp_qcert_function_to_imp_json def))
+              let (name, def) := decl in (name, imp_qcert_function_to_imp_ejson def))
            l)
     end.
 
@@ -310,16 +310,16 @@ Section ImpJsontoJavaScriptAst.
   End Lift.
 
   Section Correctness.
-    Lemma map_qcert_json_eval 
+    Lemma map_qcert_ejson_eval 
           (σ:pd_bindings) (el:list imp_expr) :
       Forall
         (fun exp : imp_expr =>
            imp_qcert_expr_eval h σ exp =
            lift_result
-             (imp_json_expr_eval (lift_pd_bindings σ) (imp_qcert_expr_to_imp_json exp))) el -> 
+             (imp_ejson_expr_eval (lift_pd_bindings σ) (imp_qcert_expr_to_imp_ejson exp))) el -> 
       map (fun x : imp_qcert_expr => imp_qcert_expr_eval h σ x) el =
       map (fun x : imp_qcert_expr => lift_result
-             (imp_json_expr_eval (lift_pd_bindings σ) (imp_qcert_expr_to_imp_json x))) el.
+             (imp_ejson_expr_eval (lift_pd_bindings σ) (imp_qcert_expr_to_imp_ejson x))) el.
     Proof.
       intros.
       apply map_eq.
@@ -331,11 +331,11 @@ Section ImpJsontoJavaScriptAst.
       destruct d; simpl; intuition discriminate.
     Qed.
     
-    Lemma data_to_bool_json_to_bool_correct j:
-      imp_qcert_data_to_bool (ejson_to_data j) = imp_json_data_to_bool j.
+    Lemma data_to_bool_ejson_to_bool_correct j:
+      imp_qcert_data_to_bool (ejson_to_data j) = imp_ejson_data_to_bool j.
     Proof.
       unfold imp_qcert_data_to_bool.
-      unfold imp_json_data_to_bool.
+      unfold imp_ejson_data_to_bool.
       destruct j; trivial.
       generalize (ejson_to_data_jobj_nbool l); intros HH1.
       match_destr.
@@ -347,11 +347,11 @@ Section ImpJsontoJavaScriptAst.
       destruct d; simpl; intuition discriminate.
     Qed.
 
-    Lemma data_to_bool_json_to_nat_correct j:
-      imp_qcert_data_to_Z (ejson_to_data j) = imp_json_data_to_Z j.
+    Lemma data_to_bool_ejson_to_nat_correct j:
+      imp_qcert_data_to_Z (ejson_to_data j) = imp_ejson_data_to_Z j.
     Proof.
       unfold imp_qcert_data_to_Z.
-      unfold imp_json_data_to_Z.
+      unfold imp_ejson_data_to_Z.
       destruct j; trivial.
       case_eq (ejson_to_data (ejobject l)); intros; try reflexivity.
       generalize (ejson_to_data_object_not_nat l z); intros.
@@ -362,9 +362,9 @@ Section ImpJsontoJavaScriptAst.
       Forall
         (fun exp : imp_expr =>
            imp_qcert_expr_eval h σ exp =
-           lift_result (imp_json_expr_eval (lift_pd_bindings σ) (imp_qcert_expr_to_imp_json exp))) [i]
+           lift_result (imp_ejson_expr_eval (lift_pd_bindings σ) (imp_qcert_expr_to_imp_ejson exp))) [i]
       -> imp_qcert_expr_eval h σ i
-         = lift_result (imp_json_expr_eval (lift_pd_bindings σ) (imp_qcert_expr_to_imp_json i)).
+         = lift_result (imp_ejson_expr_eval (lift_pd_bindings σ) (imp_qcert_expr_to_imp_ejson i)).
     Proof.
       intros.
       rewrite Forall_forall in H.
@@ -443,18 +443,24 @@ Section ImpJsontoJavaScriptAst.
       reflexivity.
     Qed.
 
-    Lemma imp_qcert_unary_op_to_imp_json_expr_correct
+    Lemma bdistinct_ejson_to_data_comm l:
+      bdistinct (map ejson_to_data l) = map ejson_to_data (bdistinct l).
+    Proof.
+      admit.
+    Admitted.
+
+    Lemma imp_qcert_unary_op_to_imp_ejson_expr_correct
            (σ:pd_bindings) (u:unary_op) (el:list imp_expr) :
       Forall
         (fun exp : imp_expr =>
            imp_qcert_expr_eval h σ exp =
            lift_result
-             (imp_json_expr_eval
-                (lift_pd_bindings σ) (imp_qcert_expr_to_imp_json exp))) el -> 
+             (imp_ejson_expr_eval
+                (lift_pd_bindings σ) (imp_qcert_expr_to_imp_ejson exp))) el -> 
       imp_qcert_expr_eval h σ (ImpExprOp (QcertOpUnary u) el) =
       lift_result
-        (imp_json_expr_eval (lift_pd_bindings σ)
-                            (imp_qcert_unary_op_to_imp_json u (map imp_qcert_expr_to_imp_json el))).
+        (imp_ejson_expr_eval (lift_pd_bindings σ)
+                            (imp_qcert_unary_op_to_imp_ejson u (map imp_qcert_expr_to_imp_ejson el))).
     Proof.
       Opaque ejson_to_data.
       intros.
@@ -473,13 +479,13 @@ Section ImpJsontoJavaScriptAst.
       (* just one param *)
       apply Forall_singleton in H.
       rewrite H; clear H.
-      unfold imp_qcert_op_eval, imp_json_op_eval.
+      unfold imp_qcert_op_eval, imp_ejson_op_eval.
       unary_op_cases (destruct u) Case; unfold lift_result, lift, olift; simpl.
       - Case "OpIdentity"%string.
-        destruct (imp_json_expr_eval (lift_pd_bindings σ) (imp_qcert_expr_to_imp_json i));
+        destruct (imp_ejson_expr_eval (lift_pd_bindings σ) (imp_qcert_expr_to_imp_ejson i));
           try reflexivity; simpl.
       - Case "OpNeg"%string.
-        destruct (imp_json_expr_eval (lift_pd_bindings σ) (imp_qcert_expr_to_imp_json i));
+        destruct (imp_ejson_expr_eval (lift_pd_bindings σ) (imp_qcert_expr_to_imp_ejson i));
           try reflexivity; simpl.
         destruct i0; try reflexivity.
         unfold unudbool.
@@ -487,29 +493,29 @@ Section ImpJsontoJavaScriptAst.
         generalize (ejson_to_data_object_not_boolean l b); intros.
         congruence.
       - Case "OpRec"%string.
-        destruct (imp_json_expr_eval (lift_pd_bindings σ) (imp_qcert_expr_to_imp_json i));
+        destruct (imp_ejson_expr_eval (lift_pd_bindings σ) (imp_qcert_expr_to_imp_ejson i));
           try reflexivity.
         simpl.
         f_equal.
         apply rec_ejson_key_encode_roundtrip.
       - Case "OpDot"%string.
-        destruct (imp_json_expr_eval (lift_pd_bindings σ) (imp_qcert_expr_to_imp_json i));
+        destruct (imp_ejson_expr_eval (lift_pd_bindings σ) (imp_qcert_expr_to_imp_ejson i));
           try reflexivity; simpl.
         destruct i0; try reflexivity; simpl.
         unfold edot.
         apply assoc_lookupr_json_key_encode_roundtrip.
       - Case "OpRecRemove"%string.
-        destruct (imp_json_expr_eval (lift_pd_bindings σ) (imp_qcert_expr_to_imp_json i));
+        destruct (imp_ejson_expr_eval (lift_pd_bindings σ) (imp_qcert_expr_to_imp_ejson i));
           try reflexivity; simpl.
         destruct i0; try reflexivity; simpl.
         apply rremove_json_key_encode_roundtrip.
       - Case "OpRecProject"%string.
         admit. (** XXX This one looks more complicated *)
       - Case "OpBag"%string.
-        destruct (imp_json_expr_eval (lift_pd_bindings σ) (imp_qcert_expr_to_imp_json i));
+        destruct (imp_ejson_expr_eval (lift_pd_bindings σ) (imp_qcert_expr_to_imp_ejson i));
           try reflexivity; simpl.
       - Case "OpSingleton"%string.
-        destruct (imp_json_expr_eval (lift_pd_bindings σ) (imp_qcert_expr_to_imp_json i));
+        destruct (imp_ejson_expr_eval (lift_pd_bindings σ) (imp_qcert_expr_to_imp_ejson i));
           try reflexivity; simpl.
         destruct i0; try reflexivity; simpl.
         + destruct l; try reflexivity; simpl.
@@ -520,7 +526,7 @@ Section ImpJsontoJavaScriptAst.
           generalize (ejson_to_data_object_not_coll l l0); intros.
           congruence.
       - Case "OpFlatten"%string.
-        destruct (imp_json_expr_eval (lift_pd_bindings σ) (imp_qcert_expr_to_imp_json i));
+        destruct (imp_ejson_expr_eval (lift_pd_bindings σ) (imp_qcert_expr_to_imp_ejson i));
           try reflexivity; simpl.
         destruct i0; try reflexivity; simpl.
         + unfold lift. simpl.
@@ -530,17 +536,25 @@ Section ImpJsontoJavaScriptAst.
           generalize (ejson_to_data_object_not_coll l l0); intros.
           congruence.
       - Case "OpDistinct"%string.
-        destruct (imp_json_expr_eval (lift_pd_bindings σ) (imp_qcert_expr_to_imp_json i));
+        destruct (imp_ejson_expr_eval (lift_pd_bindings σ) (imp_qcert_expr_to_imp_ejson i));
           try reflexivity; simpl.
         destruct i0; try reflexivity; simpl.
-        + admit.
+        + simpl.
+          unfold rondcoll.
+          unfold lift.
+          unfold ondcoll.
+          Transparent ejson_to_data.
+          simpl.
+          f_equal; f_equal.
+          Opaque ejson_to_data.
+          apply bdistinct_ejson_to_data_comm.
         + case_eq (ejson_to_data (ejobject l)); intros; try reflexivity.
           generalize (ejson_to_data_object_not_coll l l0); intros.
           congruence.
       - Case "OpOrderBy"%string.
         admit. (* XXX Not implemented *)
       - Case "OpCount"%string.
-        destruct (imp_json_expr_eval (lift_pd_bindings σ) (imp_qcert_expr_to_imp_json i));
+        destruct (imp_ejson_expr_eval (lift_pd_bindings σ) (imp_qcert_expr_to_imp_ejson i));
           try reflexivity; simpl.
         destruct i0; try reflexivity; simpl.
         + Transparent ejson_to_data. unfold ejson_to_data; simpl.
@@ -556,7 +570,7 @@ Section ImpJsontoJavaScriptAst.
       - Case "OpToText"%string.
         admit. (* XXX Not implemented *)
       - Case "OpLength"%string.
-        destruct (imp_json_expr_eval (lift_pd_bindings σ) (imp_qcert_expr_to_imp_json i));
+        destruct (imp_ejson_expr_eval (lift_pd_bindings σ) (imp_qcert_expr_to_imp_ejson i));
           try reflexivity; simpl.
         destruct i0; try reflexivity; simpl.
         case_eq (ejson_to_data (ejobject l)); intros; try reflexivity.
@@ -567,15 +581,15 @@ Section ImpJsontoJavaScriptAst.
       - Case "OpLike"%string.
         admit. (* XXX Not implemented *)
       - Case "OpLeft"%string.
-        destruct (imp_json_expr_eval (lift_pd_bindings σ) (imp_qcert_expr_to_imp_json i));
+        destruct (imp_ejson_expr_eval (lift_pd_bindings σ) (imp_qcert_expr_to_imp_ejson i));
           try reflexivity; simpl.
         destruct i0; reflexivity.
       - Case "OpRight"%string.
-        destruct (imp_json_expr_eval (lift_pd_bindings σ) (imp_qcert_expr_to_imp_json i));
+        destruct (imp_ejson_expr_eval (lift_pd_bindings σ) (imp_qcert_expr_to_imp_ejson i));
           try reflexivity; simpl.
         destruct i0; reflexivity.
       - Case "OpBrand"%string.
-        destruct (imp_json_expr_eval (lift_pd_bindings σ) (imp_qcert_expr_to_imp_json i));
+        destruct (imp_ejson_expr_eval (lift_pd_bindings σ) (imp_qcert_expr_to_imp_ejson i));
           try reflexivity; simpl.
         rewrite of_string_list_over_strings_idempotent; simpl.
         Transparent ejson_to_data.
@@ -584,7 +598,7 @@ Section ImpJsontoJavaScriptAst.
         destruct i0; try reflexivity; simpl.
         Opaque ejson_to_data.
       - Case "OpUnbrand"%string.
-        destruct (imp_json_expr_eval (lift_pd_bindings σ) (imp_qcert_expr_to_imp_json i));
+        destruct (imp_ejson_expr_eval (lift_pd_bindings σ) (imp_qcert_expr_to_imp_ejson i));
           try reflexivity; simpl.
         destruct i0; try reflexivity; simpl.
         admit. (* XXX Shouldn't be too hard with proper lemma(s) tying json_to_data and dbrand *)
@@ -618,60 +632,60 @@ Section ImpJsontoJavaScriptAst.
         admit.
     Admitted.
 
-    Lemma imp_qcert_binary_op_to_imp_json_expr_correct
+    Lemma imp_qcert_binary_op_to_imp_ejson_expr_correct
            (σ:pd_bindings) (b:binary_op) (el:list imp_expr) :
       Forall
         (fun exp : imp_expr =>
            imp_qcert_expr_eval h σ exp =
            lift_result
-             (imp_json_expr_eval
-                (lift_pd_bindings σ) (imp_qcert_expr_to_imp_json exp))) el -> 
+             (imp_ejson_expr_eval
+                (lift_pd_bindings σ) (imp_qcert_expr_to_imp_ejson exp))) el -> 
       imp_qcert_expr_eval h σ (ImpExprOp (QcertOpBinary b) el) =
       lift_result
-        (imp_json_expr_eval (lift_pd_bindings σ)
-                            (imp_qcert_binary_op_to_imp_json b (map imp_qcert_expr_to_imp_json el))).
+        (imp_ejson_expr_eval (lift_pd_bindings σ)
+                            (imp_qcert_binary_op_to_imp_ejson b (map imp_qcert_expr_to_imp_ejson el))).
     Proof.
     Admitted.
 
-    Lemma imp_qcert_runtime_call_to_imp_json_expr_correct
+    Lemma imp_qcert_runtime_call_to_imp_ejson_expr_correct
             (σ:pd_bindings) (rt:imp_qcert_runtime_op) (el:list imp_expr) :
       Forall
         (fun exp : imp_expr =>
            imp_qcert_expr_eval h σ exp =
            lift_result
-             (imp_json_expr_eval
-                (lift_pd_bindings σ) (imp_qcert_expr_to_imp_json exp))) el -> 
+             (imp_ejson_expr_eval
+                (lift_pd_bindings σ) (imp_qcert_expr_to_imp_ejson exp))) el -> 
       imp_qcert_expr_eval h σ (ImpExprRuntimeCall rt el) =
       lift_result
-        (imp_json_expr_eval (lift_pd_bindings σ)
-                            (imp_qcert_runtime_call_to_imp_json rt (map imp_qcert_expr_to_imp_json el))).
+        (imp_ejson_expr_eval (lift_pd_bindings σ)
+                            (imp_qcert_runtime_call_to_imp_ejson rt (map imp_qcert_expr_to_imp_ejson el))).
     Proof.
     Admitted.
 
-    Lemma imp_qcert_op_to_imp_json_correct
+    Lemma imp_qcert_op_to_imp_ejson_correct
           (σ:pd_bindings) (op:imp_qcert_op) (el:list imp_expr) :
       Forall
         (fun exp : imp_expr =>
            imp_qcert_expr_eval h σ exp =
            lift_result
-             (imp_json_expr_eval
-                (lift_pd_bindings σ) (imp_qcert_expr_to_imp_json exp))) el -> 
+             (imp_ejson_expr_eval
+                (lift_pd_bindings σ) (imp_qcert_expr_to_imp_ejson exp))) el -> 
       imp_qcert_expr_eval h σ (ImpExprOp op el) =
       lift_result
-        (imp_json_expr_eval (lift_pd_bindings σ)
-                            (imp_qcert_op_to_imp_json op (map imp_qcert_expr_to_imp_json el))).
+        (imp_ejson_expr_eval (lift_pd_bindings σ)
+                            (imp_qcert_op_to_imp_ejson op (map imp_qcert_expr_to_imp_ejson el))).
     Proof.
       intros.
       destruct op.
-      + apply imp_qcert_unary_op_to_imp_json_expr_correct; assumption.
-      + apply imp_qcert_binary_op_to_imp_json_expr_correct; assumption.
+      + apply imp_qcert_unary_op_to_imp_ejson_expr_correct; assumption.
+      + apply imp_qcert_binary_op_to_imp_ejson_expr_correct; assumption.
     Qed.
 
-    Lemma imp_qcert_expr_to_imp_json_expr_correct (σ:pd_bindings) (exp:imp_qcert_expr) :
+    Lemma imp_qcert_expr_to_imp_ejson_expr_correct (σ:pd_bindings) (exp:imp_qcert_expr) :
       imp_qcert_expr_eval h σ exp =
       lift_result
-        (imp_json_expr_eval (lift_pd_bindings σ)
-                            (imp_qcert_expr_to_imp_json exp)).
+        (imp_ejson_expr_eval (lift_pd_bindings σ)
+                            (imp_qcert_expr_to_imp_ejson exp)).
     Proof.
       imp_expr_cases (induction exp) Case.
       - Case "ImpExprError"%string.
@@ -691,35 +705,37 @@ Section ImpJsontoJavaScriptAst.
         simpl.
         f_equal.
         unfold imp_qcert_data_normalize.
-        unfold imp_json_data_normalize.
+        unfold imp_ejson_data_normalize.
         rewrite json_to_data_to_json_idempotent.
         reflexivity.
       - Case "ImpExprOp"%string.
-        apply imp_qcert_op_to_imp_json_correct; assumption.
+        apply imp_qcert_op_to_imp_ejson_correct; assumption.
       - Case "ImpExprRuntimeCall"%string.
-        apply imp_qcert_runtime_call_to_imp_json_expr_correct; assumption.
+        apply imp_qcert_runtime_call_to_imp_ejson_expr_correct; assumption.
     Qed.
 
-    Lemma imp_qcert_stmt_to_imp_json_stmt_correct (σ:pd_bindings) (stmt:imp_qcert_stmt) :
+    Lemma imp_qcert_stmt_to_imp_ejson_stmt_correct (σ:pd_bindings) (stmt:imp_qcert_stmt) :
       forall avoid: list string,
          (* (fres_var stmt) avoid -> *)
         imp_qcert_stmt_eval h stmt σ =
-        lift_result_env (imp_json_stmt_eval (imp_qcert_stmt_to_imp_json avoid stmt) (lift_pd_bindings σ)).
+        lift_result_env (imp_ejson_stmt_eval (imp_qcert_stmt_to_imp_ejson avoid stmt) (lift_pd_bindings σ)).
     Proof.
       imp_stmt_cases (induction stmt) Case.
       - Case "ImpStmtBlock"%string.
+        intros.
+        (* XXX. Someing wrong here, missing inductive principle on imp statements. *)
         admit.
       - Case "ImpStmtAssign"%string.
         intros avoid.
         simpl.
-        specialize (imp_qcert_expr_to_imp_json_expr_correct σ i).
+        specialize (imp_qcert_expr_to_imp_ejson_expr_correct σ i).
         unfold imp_qcert_expr_eval in *.
         intros Hi.
         rewrite Hi.
         unfold lift_result.
         unfold lift.
-        unfold imp_json_expr_eval.
-        destruct (ImpEval.imp_expr_eval (lift_pd_bindings σ) (imp_qcert_expr_to_imp_json i));
+        unfold imp_ejson_expr_eval.
+        destruct (ImpEval.imp_expr_eval (lift_pd_bindings σ) (imp_qcert_expr_to_imp_ejson i));
           try reflexivity.
         unfold lift_pd_bindings.
         rewrite lookup_map_codomain_unfolded.
@@ -750,6 +766,15 @@ Section ImpJsontoJavaScriptAst.
           rewrite json_to_data_to_json_idempotent.
           reflexivity.
       - Case "ImpStmtFor"%string.
+        intros avoid.
+        specialize (imp_qcert_expr_to_imp_ejson_expr_correct σ i); simpl; unfold imp_qcert_expr_eval; intros.
+        rewrite H; clear H.
+        unfold lift_result; simpl.
+        unfold imp_ejson_expr_eval; simpl.
+        unfold lift; simpl.
+        destruct (ImpEval.imp_expr_eval (lift_pd_bindings σ) (imp_qcert_expr_to_imp_ejson i));
+          simpl; [|reflexivity].
+        (* XXX. Someing wrong here, likely translation to for-range variant always fails. *)
         admit.
       - Case "ImpStmtForRange"%string.
         intros avoid.
@@ -757,41 +782,41 @@ Section ImpJsontoJavaScriptAst.
       - Case "ImpStmtIf"%string.
         intros avoid.
         simpl.
-        specialize (imp_qcert_expr_to_imp_json_expr_correct σ i).
+        specialize (imp_qcert_expr_to_imp_ejson_expr_correct σ i).
         unfold imp_qcert_expr_eval in *.
         intros Hi.
         rewrite Hi.
         unfold lift_result.
         unfold lift.
-        unfold imp_json_expr_eval.
-        destruct (ImpEval.imp_expr_eval (lift_pd_bindings σ) (imp_qcert_expr_to_imp_json i));
+        unfold imp_ejson_expr_eval.
+        destruct (ImpEval.imp_expr_eval (lift_pd_bindings σ) (imp_qcert_expr_to_imp_ejson i));
           try reflexivity.
-        rewrite data_to_bool_json_to_bool_correct.
+        rewrite data_to_bool_ejson_to_bool_correct.
         match_destr.
         match_destr.
     (* Qed. *)
     Admitted.
 
-    Lemma imp_qcert_function_to_imp_json_function_correct (d:data) (f:imp_qcert_function) :
+    Lemma imp_qcert_function_to_imp_ejson_function_correct (d:data) (f:imp_qcert_function) :
       imp_qcert_function_eval h f d =
-      lift ejson_to_data (imp_json_function_eval (imp_qcert_function_to_imp_json f) (data_to_ejson d)).
+      lift ejson_to_data (imp_ejson_function_eval (imp_qcert_function_to_imp_ejson f) (data_to_ejson d)).
     Proof.
       destruct f; simpl.
-      generalize (imp_qcert_stmt_to_imp_json_stmt_correct [(v0, None); (v, Some d)] i (v::nil)); intros.
+      generalize (imp_qcert_stmt_to_imp_ejson_stmt_correct [(v0, None); (v, Some d)] i (v::nil)); intros.
       unfold imp_qcert_stmt_eval in H.
-      unfold imp_json_stmt_eval in H.
+      unfold imp_ejson_stmt_eval in H.
       unfold imp_qcert_data in *.
       rewrite H; clear H.
       unfold lift_result_env.
       unfold lift.
-      case_eq (@ImpEval.imp_stmt_eval _ _ _ imp_json_data_normalize imp_json_data_to_bool imp_json_data_to_Z imp_json_data_to_list imp_json_Z_to_data imp_json_runtime_eval imp_json_op_eval (imp_qcert_stmt_to_imp_json [v] i) (lift_pd_bindings [(v0, None); (v, Some d)])); intros.
+      case_eq (@ImpEval.imp_stmt_eval _ _ _ imp_ejson_data_normalize imp_ejson_data_to_bool imp_ejson_data_to_Z imp_ejson_data_to_list imp_ejson_Z_to_data imp_ejson_runtime_eval imp_ejson_op_eval (imp_qcert_stmt_to_imp_ejson [v] i) (lift_pd_bindings [(v0, None); (v, Some d)])); intros.
       - unfold olift.
-        unfold imp_json_data in *.
+        unfold imp_ejson_data in *.
         unfold imp_qcert_data in *.
-        unfold imp_json_op in *.
-        assert ((@ImpEval.imp_stmt_eval ejson ejson_op imp_json_runtime_op imp_json_data_normalize imp_json_data_to_bool
-           imp_json_data_to_Z imp_json_data_to_list imp_json_Z_to_data imp_json_runtime_eval imp_json_op_eval
-           (imp_qcert_stmt_to_imp_json (@cons var v (@nil var)) i)
+        unfold imp_ejson_op in *.
+        assert ((@ImpEval.imp_stmt_eval ejson ejson_op imp_ejson_runtime_op imp_ejson_data_normalize imp_ejson_data_to_bool
+           imp_ejson_data_to_Z imp_ejson_data_to_list imp_ejson_Z_to_data imp_ejson_runtime_eval imp_ejson_op_eval
+           (imp_qcert_stmt_to_imp_ejson (@cons var v (@nil var)) i)
            (lift_pd_bindings
               (@cons (prod var (option (@data (@foreign_runtime_data fruntime))))
                  (@pair var (option (@data (@foreign_runtime_data fruntime))) v0
@@ -800,9 +825,9 @@ Section ImpJsontoJavaScriptAst.
                     (@pair var (option (@data (@foreign_runtime_data fruntime))) v
                        (@Some (@data (@foreign_runtime_data fruntime)) d))
                     (@nil (prod var (option (@data (@foreign_runtime_data fruntime)))))))))
-                = (@ImpEval.imp_stmt_eval ejson ejson_op imp_json_runtime_op imp_json_data_normalize imp_json_data_to_bool
-          imp_json_data_to_Z imp_json_data_to_list imp_json_Z_to_data imp_json_runtime_eval imp_json_op_eval
-          (imp_qcert_stmt_to_imp_json (@cons var v (@nil var)) i)
+                = (@ImpEval.imp_stmt_eval ejson ejson_op imp_ejson_runtime_op imp_ejson_data_normalize imp_ejson_data_to_bool
+          imp_ejson_data_to_Z imp_ejson_data_to_list imp_ejson_Z_to_data imp_ejson_runtime_eval imp_ejson_op_eval
+          (imp_qcert_stmt_to_imp_ejson (@cons var v (@nil var)) i)
           (@cons (prod var (option ejson)) (@pair var (option ejson) v0 (@None ejson))
              (@cons (prod var (option ejson))
                 (@pair var (option ejson) v (@Some ejson (@data_to_ejson (@foreign_runtime_data fruntime) _ ftejson d)))
@@ -819,12 +844,12 @@ Section ImpJsontoJavaScriptAst.
         rewrite H; clear H.
         case_eq (lookup EquivDec.equiv_dec p v0); intros; try reflexivity.
       - unfold olift.
-        unfold imp_json_data in *.
+        unfold imp_ejson_data in *.
         unfold imp_qcert_data in *.
-        unfold imp_json_op in *.
-        assert ((@ImpEval.imp_stmt_eval ejson ejson_op imp_json_runtime_op imp_json_data_normalize imp_json_data_to_bool
-           imp_json_data_to_Z imp_json_data_to_list imp_json_Z_to_data imp_json_runtime_eval imp_json_op_eval
-           (imp_qcert_stmt_to_imp_json (@cons var v (@nil var)) i)
+        unfold imp_ejson_op in *.
+        assert ((@ImpEval.imp_stmt_eval ejson ejson_op imp_ejson_runtime_op imp_ejson_data_normalize imp_ejson_data_to_bool
+           imp_ejson_data_to_Z imp_ejson_data_to_list imp_ejson_Z_to_data imp_ejson_runtime_eval imp_ejson_op_eval
+           (imp_qcert_stmt_to_imp_ejson (@cons var v (@nil var)) i)
            (lift_pd_bindings
               (@cons (prod var (option (@data (@foreign_runtime_data fruntime))))
                  (@pair var (option (@data (@foreign_runtime_data fruntime))) v0
@@ -833,9 +858,9 @@ Section ImpJsontoJavaScriptAst.
                     (@pair var (option (@data (@foreign_runtime_data fruntime))) v
                        (@Some (@data (@foreign_runtime_data fruntime)) d))
                     (@nil (prod var (option (@data (@foreign_runtime_data fruntime)))))))))
-                = (@ImpEval.imp_stmt_eval ejson ejson_op imp_json_runtime_op imp_json_data_normalize imp_json_data_to_bool
-          imp_json_data_to_Z imp_json_data_to_list imp_json_Z_to_data imp_json_runtime_eval imp_json_op_eval
-          (imp_qcert_stmt_to_imp_json (@cons var v (@nil var)) i)
+                = (@ImpEval.imp_stmt_eval ejson ejson_op imp_ejson_runtime_op imp_ejson_data_normalize imp_ejson_data_to_bool
+          imp_ejson_data_to_Z imp_ejson_data_to_list imp_ejson_Z_to_data imp_ejson_runtime_eval imp_ejson_op_eval
+          (imp_qcert_stmt_to_imp_ejson (@cons var v (@nil var)) i)
           (@cons (prod var (option ejson)) (@pair var (option ejson) v0 (@None ejson))
              (@cons (prod var (option ejson))
                 (@pair var (option ejson) v (@Some ejson (@data_to_ejson (@foreign_runtime_data fruntime) _ ftejson d)))
@@ -854,27 +879,27 @@ Section ImpJsontoJavaScriptAst.
       - intros; split; intros; auto.
     Qed.
 
-    Theorem imp_qcert_to_imp_json_correct (σc:bindings) (q:imp_qcert) :
+    Theorem imp_qcert_to_imp_ejson_correct (σc:bindings) (q:imp_qcert) :
       imp_qcert_eval_top h σc q =
-      imp_json_eval_top_alt σc (imp_qcert_to_imp_json q).
+      imp_ejson_eval_top σc (imp_qcert_to_imp_ejson q).
     Proof.
       unfold imp_qcert_eval_top.
-      unfold imp_json_eval_top_alt.
-      unfold imp_json_eval_top.
-      unfold imp_json_eval.
+      unfold imp_ejson_eval_top.
+      unfold imp_ejson_eval_top_on_ejson.
+      unfold imp_ejson_eval.
       destruct q; simpl.
       destruct l; try reflexivity; simpl.
       destruct p; simpl.
       destruct l; try reflexivity; simpl.
-      generalize (imp_qcert_function_to_imp_json_function_correct (drec (rec_sort σc)) i); intros.
+      generalize (imp_qcert_function_to_imp_ejson_function_correct (drec (rec_sort σc)) i); intros.
       unfold imp_qcert_eval_top.
-      unfold imp_json_eval_top_alt.
-      unfold imp_json_eval_top.
-      unfold imp_json_eval.
+      unfold imp_ejson_eval_top.
+      unfold imp_ejson_eval_top_on_ejson.
+      unfold imp_ejson_eval.
       unfold id; simpl.
       simpl in H.
       unfold imp_qcert_function_eval in H.
-      unfold imp_json_function_eval in H.
+      unfold imp_ejson_function_eval in H.
       rewrite H; clear H.
       f_equal.
       f_equal.
@@ -886,4 +911,4 @@ Section ImpJsontoJavaScriptAst.
 
   End Correctness.
 
-End ImpJsontoJavaScriptAst.
+End ImpQcerttoImpEJson.
