compiler/src/Compiler/Driver/CompCorrectness.v
@@ -71,7 +71,7 @@ Require Import NNRCtoDNNRC.
 Require Import NNRCtoNNRCMR.
 Require Import NNRStoNNRSimp.
 Require Import NNRSimptoImpQcert.
-Require Import ImpQcerttoImpJson.
+Require Import ImpQcerttoImpEJson.
 Require Import NNRCtoJava.
 Require Import cNNRCtoCAMP.
 Require Import cNNRCtoNNRC.
@@ -93,7 +93,7 @@ Require Import OptimizerLogger.
 Require Import ForeignToReduceOps.
 Require Import ForeignToSpark.
 Require Import ForeignToJava.
-Require Import ForeignEJSONtoJavaScriptAst.
+Require Import ForeignToJavaScriptAst.
 Require Import ForeignToScala.
 
 (** Compiler Driver *)
@@ -120,7 +120,7 @@ Section CompCorrectness.
   Context {nnrs_imp_stmt_logger:optimizer_logger string nnrs_imp_stmt}.
   Context {nnrs_imp_logger:optimizer_logger string nnrs_imp}.
   Context {imp_qcert_logger:optimizer_logger string imp_qcert}.
-  Context {imp_json_logger:optimizer_logger string imp_json}.
+  Context {imp_ejson_logger:optimizer_logger string imp_ejson}.
   Context {dnnrc_logger:optimizer_logger string (DNNRCBase.dnnrc_base fr (type_annotation unit) dataframe)}.
   Context {ftojava:foreign_to_java}.
   Context {ftos:foreign_to_scala}.
@@ -166,16 +166,16 @@ Section CompCorrectness.
     | Dv_dnnrc_to_dnnrc_typed _ dv => False /\ driver_correct_dnnrc_typed dv
     end.
 
-  Fixpoint driver_correct_imp_json (dv: imp_json_driver) :=
+  Fixpoint driver_correct_imp_ejson (dv: imp_ejson_driver) :=
     match dv with
-    | Dv_imp_json_stop => True
-    | Dv_imp_json_to_js_ast dv => False /\ driver_correct_js_ast dv
+    | Dv_imp_ejson_stop => True
+    | Dv_imp_ejson_to_js_ast dv => False /\ driver_correct_js_ast dv
     end.
 
   Fixpoint driver_correct_imp_qcert (dv: imp_qcert_driver) :=
     match dv with
     | Dv_imp_qcert_stop => True
-    | Dv_imp_qcert_to_imp_json dv => False /\ driver_correct_imp_json dv
+    | Dv_imp_qcert_to_imp_ejson dv => False /\ driver_correct_imp_ejson dv
     end.
 
   Fixpoint driver_correct_nnrs_imp (dv: nnrs_imp_driver) :=
@@ -316,7 +316,7 @@ Section CompCorrectness.
     | Dv_nnrs dv => driver_correct_nnrs dv
     | Dv_nnrs_imp dv => driver_correct_nnrs_imp dv
     | Dv_imp_qcert dv => driver_correct_imp_qcert dv
-    | Dv_imp_json dv => driver_correct_imp_json dv
+    | Dv_imp_ejson dv => driver_correct_imp_ejson dv
     | Dv_nnrcmr dv => driver_correct_nnrcmr dv
     | Dv_dnnrc dv => driver_correct_dnnrc dv
     | Dv_dnnrc_typed dv => driver_correct_dnnrc_typed dv
@@ -347,7 +347,7 @@ Section CompCorrectness.
     Ltac prove_same_outputs :=
       unfold eval_camp_rule, eval_camp,
       eval_nra, eval_nraenv, eval_nraenv_core,
-      eval_nnrc, eval_nnrc_core, eval_nnrs, eval_nnrs_imp, eval_imp_qcert, eval_imp_json, eval_nnrcmr,
+      eval_nnrc, eval_nnrc_core, eval_nnrs, eval_nnrs_imp, eval_imp_qcert, eval_imp_ejson, eval_nnrcmr,
       eval_dnnrc, eval_dnnrc_typed;
       try match goal with
       | [ |- equal_outputs (lift_output (camp_rule_eval_top ?h ?c (lift_input ?i)))
@@ -439,7 +439,7 @@ Section CompCorrectness.
     | (Dv_nnrs _, Q_nnrs _) => True
     | (Dv_nnrs_imp _, Q_nnrs_imp _) => True
     | (Dv_imp_qcert _, Q_imp_qcert _) => True
-    | (Dv_imp_json _, Q_imp_json _) => True
+    | (Dv_imp_ejson _, Q_imp_ejson _) => True
     | (Dv_nnrcmr _, Q_nnrcmr _) => True
     | (Dv_dnnrc _, Q_dnnrc _) => True
     | (Dv_dnnrc_typed _, Q_dnnrc_typed _) => True
@@ -450,10 +450,10 @@ Section CompCorrectness.
     | (_, _) => False
     end.
 
-    Lemma correct_driver_succeeds_imp_json:
-      forall dv, driver_correct (Dv_imp_json dv) ->
+    Lemma correct_driver_succeeds_imp_ejson:
+      forall dv, driver_correct (Dv_imp_ejson dv) ->
                  (forall q, Forall query_not_error
-                                   (compile (Dv_imp_json dv) (Q_imp_json q))).
+                                   (compile (Dv_imp_ejson dv) (Q_imp_ejson q))).
     Proof.
       intros.
       rewrite Forall_forall; intros.
@@ -946,7 +946,7 @@ Section CompCorrectness.
       - apply correct_driver_succeeds_nnrs; auto.
       - apply correct_driver_succeeds_nnrs_imp; auto.
       - apply correct_driver_succeeds_imp_qcert; auto.
-      - apply correct_driver_succeeds_imp_json; auto.
+      - apply correct_driver_succeeds_imp_ejson; auto.
       - apply correct_driver_succeeds_nnrcmr; auto.
       - apply correct_driver_succeeds_dnnrc; auto.
       - apply correct_driver_succeeds_dnnrc_typed; auto.
@@ -1304,10 +1304,10 @@ Section CompCorrectness.
       trivial_same_query.
     Qed.
 
-    Lemma correct_driver_preserves_eval_imp_json:
-      forall dv, driver_correct (Dv_imp_json dv) ->
-                 (forall q, Forall (query_preserves_eval (Q_imp_json q))
-                                   (compile (Dv_imp_json dv) (Q_imp_json q))).
+    Lemma correct_driver_preserves_eval_imp_ejson:
+      forall dv, driver_correct (Dv_imp_ejson dv) ->
+                 (forall q, Forall (query_preserves_eval (Q_imp_ejson q))
+                                   (compile (Dv_imp_ejson dv) (Q_imp_ejson q))).
     Proof.
       intros.
       rewrite Forall_forall; intros.
@@ -1962,7 +1962,7 @@ input data returns the same output data. *)
       - apply correct_driver_preserves_eval_nnrs; auto.
       - apply correct_driver_preserves_eval_nnrs_imp; auto.
       - apply correct_driver_preserves_eval_imp_qcert; auto.
-      - apply correct_driver_preserves_eval_imp_json; auto.
+      - apply correct_driver_preserves_eval_imp_ejson; auto.
       - apply correct_driver_preserves_eval_nnrcmr; auto.
       - apply correct_driver_preserves_eval_dnnrc; auto.
       - apply correct_driver_preserves_eval_dnnrc_typed; auto.
