compiler/src/Compiler/Model/CompilerRuntime.v
@@ -17,9 +17,9 @@
 Require Import String.
 Require Import CommonRuntime.
 Require Import ForeignToJava.
-Require Import ForeignEJSONtoJavaScriptAst.
+Require Import ForeignToJavaScriptAst.
 Require Import ForeignToScala.
-Require Import ForeignDataToEJSON.
+Require Import ForeignDataToEJson.
 Require Import ForeignTypeToJSON.
 Require Import ForeignReduceOps.
 Require Import ForeignToReduceOps.
