compiler/src/Imp/Lang/ImpEJson.v
@@ -1,0 +1,145 @@
+(*
+ * Copyright 2015-2016 IBM Corporation
+ *
+ * Licensed under the Apache License, Version 2.0 (the "License");
+ * you may not use this file except in compliance with the License.
+ * You may obtain a copy of the License at
+ *
+ * http://www.apache.org/licenses/LICENSE-2.0
+ *
+ * Unless required by applicable law or agreed to in writing, software
+ * distributed under the License is distributed on an "AS IS" BASIS,
+ * WITHOUT WARRANTIES OR CONDITIONS OF ANY KIND, either express or implied.
+ * See the License for the specific language governing permissions and
+ * limitations under the License.
+ *)
+
+(** Imp with the Json data model *)
+
+Require Import String.
+Require Import CommonRuntime.
+Require Import Imp.
+
+Section ImpEJson.
+  Section Syntax.
+    Context {ftoejson:foreign_ejson}.
+
+    Definition imp_ejson_data := ejson.
+
+    (* XXX This should contain at least:
+       - all JS operators/expressions used in translation from NNRSimp to JsAst
+       - all JS operators/expressions used to manipulate values in data but not in json (brands, nat, left, right, foreign)
+       imp_ejson_op constructors names are based on JsAst names
+       imp_ejson_runtime_op constructors namess are based on Qcert operators names ??
+     *)
+    Definition imp_ejson_op := ejson_op. (* See ./Common/EJson/EJsonOperators.v *)
+    Inductive imp_ejson_runtime_op := (* XXX TODO -- Look at NNRSimptoJavaScriptAst XXX *)
+    | EJsonRuntimeEqual : imp_ejson_runtime_op
+    | EJsonRuntimeCompare : imp_ejson_runtime_op
+    | EJsonRuntimeRecConcat : imp_ejson_runtime_op
+    | EJsonRuntimeRecMerge : imp_ejson_runtime_op
+    | EJsonRuntimeDistinct : imp_ejson_runtime_op
+    | EJsonRuntimeGroupBy : imp_ejson_runtime_op
+    | EJsonRuntimeDeref : imp_ejson_runtime_op
+    | EJsonRuntimeEither : imp_ejson_runtime_op
+    | EJsonRuntimeToLeft: imp_ejson_runtime_op
+    | EJsonRuntimeToRight: imp_ejson_runtime_op
+    | EJsonRuntimeRemove: imp_ejson_runtime_op
+    | EJsonRuntimeProject: imp_ejson_runtime_op
+    | EJsonRuntimeSingleton : imp_ejson_runtime_op
+    | EJsonRuntimeFlatten : imp_ejson_runtime_op
+    | EJsonRuntimeSort : imp_ejson_runtime_op
+    | EJsonRuntimeCount : imp_ejson_runtime_op
+    | EJsonRuntimeLength : imp_ejson_runtime_op
+    | EJsonRuntimeSubstring : imp_ejson_runtime_op
+    | EJsonRuntimeBrand : imp_ejson_runtime_op
+    | EJsonRuntimeUnbrand : imp_ejson_runtime_op
+    | EJsonRuntimeCast : imp_ejson_runtime_op
+    | EJsonRuntimeNatPlus : imp_ejson_runtime_op
+    | EJsonRuntimeNatMinus : imp_ejson_runtime_op
+    | EJsonRuntimeNatMult : imp_ejson_runtime_op
+    | EJsonRuntimeNatDiv : imp_ejson_runtime_op
+    | EJsonRuntimeNatRem : imp_ejson_runtime_op
+    | EJsonRuntimeNatAbs : imp_ejson_runtime_op
+    | EJsonRuntimeNatLog2 : imp_ejson_runtime_op
+    | EJsonRuntimeNatSqrt : imp_ejson_runtime_op
+    | EJsonRuntimeNatSum : imp_ejson_runtime_op
+    | EJsonRuntimeNatMin : imp_ejson_runtime_op
+    | EJsonRuntimeNatMax : imp_ejson_runtime_op
+    | EJsonRuntimeNatArithMean : imp_ejson_runtime_op
+    | EJsonRuntimeFloatOfNat : imp_ejson_runtime_op
+    | EJsonRuntimeSum : imp_ejson_runtime_op
+    | EJsonRuntimeArithMean : imp_ejson_runtime_op
+    | EJsonRuntimeBunion : imp_ejson_runtime_op
+    | EJsonRuntimeBminus : imp_ejson_runtime_op
+    | EJsonRuntimeBmin : imp_ejson_runtime_op
+    | EJsonRuntimeBmax : imp_ejson_runtime_op
+    | EJsonRuntimeBnth : imp_ejson_runtime_op
+    | EJsonRuntimeContains : imp_ejson_runtime_op
+    | EJsonRuntimeStringJoin : imp_ejson_runtime_op
+    | EJsonRuntimeToString : imp_ejson_runtime_op
+    | EJsonRuntimeToText : imp_ejson_runtime_op
+    .
+
+    Definition imp_ejson_expr := @imp_expr imp_ejson_data imp_ejson_op imp_ejson_runtime_op.
+    Definition imp_ejson_stmt := @imp_stmt imp_ejson_data imp_ejson_op imp_ejson_runtime_op.
+    Definition imp_ejson_function := @imp_function imp_ejson_data imp_ejson_op imp_ejson_runtime_op.
+    Definition imp_ejson := @imp imp_ejson_data imp_ejson_op imp_ejson_runtime_op.
+
+  End Syntax.
+
+  Section Util.
+
+    Local Open Scope string.
+
+    Definition string_of_ejson_runtime_op (op: imp_ejson_runtime_op) :=
+      match op with
+      | EJsonRuntimeEqual => "equal"
+      | EJsonRuntimeCompare => "compare"
+      | EJsonRuntimeRecConcat => "concat"
+      | EJsonRuntimeRecMerge => "mergeConcat"
+      | EJsonRuntimeDistinct => "distinct"
+      | EJsonRuntimeGroupBy => "groupBy" (* XXX TODO: to check XXX *)
+      | EJsonRuntimeDeref => "deref"
+      | EJsonRuntimeEither => "either"
+      | EJsonRuntimeToLeft=> "toLeft"
+      | EJsonRuntimeToRight=> "toRight"
+      | EJsonRuntimeRemove=> "remove"
+      | EJsonRuntimeProject=> "project"
+      | EJsonRuntimeSingleton => "singleton"
+      | EJsonRuntimeFlatten => "flatten"
+      | EJsonRuntimeSort => "sort"
+      | EJsonRuntimeCount => "count"
+      | EJsonRuntimeLength => "stringLength"
+      | EJsonRuntimeSubstring => "substring"
+      | EJsonRuntimeBrand => "brand"
+      | EJsonRuntimeUnbrand => "unbrand"
+      | EJsonRuntimeCast => "cast"
+      | EJsonRuntimeNatPlus => "natPlus"
+      | EJsonRuntimeNatMinus => "natMinus"
+      | EJsonRuntimeNatMult => "natMult"
+      | EJsonRuntimeNatDiv => "natDiv"
+      | EJsonRuntimeNatRem => "natRem"
+      | EJsonRuntimeNatAbs => "natAbs"
+      | EJsonRuntimeNatLog2 => "natLog2"
+      | EJsonRuntimeNatSqrt => "natSqrt"
+      | EJsonRuntimeNatSum => "natSum"
+      | EJsonRuntimeNatMin => "natMin"
+      | EJsonRuntimeNatMax => "natMax"
+      | EJsonRuntimeNatArithMean => "natArithMean"
+      | EJsonRuntimeFloatOfNat => "floatOfNat"
+      | EJsonRuntimeSum => "sum"
+      | EJsonRuntimeArithMean => "arithMean"
+      | EJsonRuntimeBunion => "bunion"
+      | EJsonRuntimeBminus => "bminus"
+      | EJsonRuntimeBmin => "bmin"
+      | EJsonRuntimeBmax => "bmax"
+      | EJsonRuntimeBnth => "bnth"
+      | EJsonRuntimeContains => "contains"
+      | EJsonRuntimeStringJoin => "stringJoin"
+      | EJsonRuntimeToString => "toString"
+      | EJsonRuntimeToText => "toText"
+      end.
+
+  End Util.
+End ImpEJson.
