compiler/src/Translation/ImpEJsontoJavaScriptAst.v
@@ -20,11 +20,11 @@ Require Import Bool.
 Require Import Arith.
 Require Import Utils.
 Require Import Imp.
-Require Import ImpJson.
+Require Import ImpEJson.
 Require Import JavaScriptAstRuntime.
-Require Import ForeignEJSONtoJavaScriptAst.
+Require Import ForeignToJavaScriptAst.
 
-Section ImpJsontoJavaScriptAst.
+Section ImpEJsontoJavaScriptAst.
   Import ListNotations.
 
   Section Util.
@@ -62,53 +62,53 @@ Section ImpJsontoJavaScriptAst.
       | None => mk_expr_error
       end.
 
-    Definition mk_runtime_call (op: imp_json_runtime_op) (el: list expr) :=
-      call_runtime (string_of_json_runtime_op op) el.
+    Definition mk_runtime_call (op: imp_ejson_runtime_op) (el: list expr) :=
+      call_runtime (string_of_ejson_runtime_op op) el.
 
-    Definition imp_json_op_to_js_ast (op:imp_json_op) el : expr :=
+    Definition imp_ejson_op_to_js_ast (op:imp_ejson_op) el : expr :=
       match op with
-      | EJSONOpNot => mk_unary_op unary_op_not el
-      | EJSONOpNeg => mk_unary_op unary_op_neg el
-      | EJSONOpAnd => mk_binary_op binary_op_and el
-      | EJSONOpOr => mk_binary_op binary_op_or el
-      | EJSONOpLt => mk_binary_op binary_op_lt el
-      | EJSONOpLe => mk_binary_op binary_op_le el
-      | EJSONOpGt => mk_binary_op binary_op_gt el
-      | EJSONOpGe => mk_binary_op binary_op_ge el
-      | EJSONOpAddString => mk_binary_op binary_op_add el
-      | EJSONOpAddNumber => mk_binary_op binary_op_add el
-      | EJSONOpSub => mk_binary_op binary_op_sub el
-      | EJSONOpDiv => mk_binary_op binary_op_div el
-      | EJSONOpMult => mk_binary_op binary_op_mult el
-      | EJSONOpStrictEqual => mk_binary_op binary_op_strict_equal el
-      | EJSONOpStrictDisequal => mk_binary_op binary_op_strict_disequal el
-      | EJSONOpArray => expr_array (List.map Some el)
-      | EJSONOpArrayLength => mk_unary_expr (fun e => expr_member e  "length") el
-      | EJSONOpArrayPush => mk_binary_expr array_push el
-      | EJSONOpArrayAccess => mk_binary_expr array_get el
-      | EJSONOpObject atts => mk_object atts el
-      | EJSONOpAccess att => mk_binary_expr expr_access (el++[expr_literal (literal_string att)])
-      | EJSONOpHasOwnProperty att => mk_binary_expr object_hasOwnProperty (el++[expr_literal (literal_string att)])
-      | EJSONOpToString => expr_call (expr_identifier "toString") el
-      | EJSONOpMathMin => expr_call (expr_member (expr_identifier "Math") "min") el
-      | EJSONOpMathMax => expr_call (expr_member (expr_identifier "Math") "max") el
-      | EJSONOpMathMinApply =>
+      | EJsonOpNot => mk_unary_op unary_op_not el
+      | EJsonOpNeg => mk_unary_op unary_op_neg el
+      | EJsonOpAnd => mk_binary_op binary_op_and el
+      | EJsonOpOr => mk_binary_op binary_op_or el
+      | EJsonOpLt => mk_binary_op binary_op_lt el
+      | EJsonOpLe => mk_binary_op binary_op_le el
+      | EJsonOpGt => mk_binary_op binary_op_gt el
+      | EJsonOpGe => mk_binary_op binary_op_ge el
+      | EJsonOpAddString => mk_binary_op binary_op_add el
+      | EJsonOpAddNumber => mk_binary_op binary_op_add el
+      | EJsonOpSub => mk_binary_op binary_op_sub el
+      | EJsonOpDiv => mk_binary_op binary_op_div el
+      | EJsonOpMult => mk_binary_op binary_op_mult el
+      | EJsonOpStrictEqual => mk_binary_op binary_op_strict_equal el
+      | EJsonOpStrictDisequal => mk_binary_op binary_op_strict_disequal el
+      | EJsonOpArray => expr_array (List.map Some el)
+      | EJsonOpArrayLength => mk_unary_expr (fun e => expr_member e  "length") el
+      | EJsonOpArrayPush => mk_binary_expr array_push el
+      | EJsonOpArrayAccess => mk_binary_expr array_get el
+      | EJsonOpObject atts => mk_object atts el
+      | EJsonOpAccess att => mk_binary_expr expr_access (el++[expr_literal (literal_string att)])
+      | EJsonOpHasOwnProperty att => mk_binary_expr object_hasOwnProperty (el++[expr_literal (literal_string att)])
+      | EJsonOpToString => expr_call (expr_identifier "toString") el
+      | EJsonOpMathMin => expr_call (expr_member (expr_identifier "Math") "min") el
+      | EJsonOpMathMax => expr_call (expr_member (expr_identifier "Math") "max") el
+      | EJsonOpMathMinApply =>
         expr_call
           (expr_member (expr_member (expr_identifier "Math") "min") "apply")
           (expr_identifier "Math" :: el)
-      | EJSONOpMathMaxApply =>
+      | EJsonOpMathMaxApply =>
         expr_call
           (expr_member (expr_member (expr_identifier "Math") "max") "apply")
           (expr_identifier "Math" :: el)
-      | EJSONOpMathPow => expr_call (expr_member (expr_identifier "Math") "pow") el
-      | EJSONOpMathExp => expr_call (expr_member (expr_identifier "Math") "exp") el
-      | EJSONOpMathAbs => expr_call (expr_member (expr_identifier "Math") "abs") el
-      | EJSONOpMathLog => expr_call (expr_member (expr_identifier "Math") "log2") el
-      | EJSONOpMathLog10 => expr_call (expr_member (expr_identifier "Math") "log10") el
-      | EJSONOpMathSqrt => expr_call (expr_member (expr_identifier "Math") "sqrt") el
-      | EJSONOpMathCeil => expr_call (expr_member (expr_identifier "Math") "ceil") el
-      | EJSONOpMathFloor => expr_call (expr_member (expr_identifier "Math") "floor") el
-      | EJSONOpMathTrunc => expr_call (expr_member (expr_identifier "Math") "trunc") el
+      | EJsonOpMathPow => expr_call (expr_member (expr_identifier "Math") "pow") el
+      | EJsonOpMathExp => expr_call (expr_member (expr_identifier "Math") "exp") el
+      | EJsonOpMathAbs => expr_call (expr_member (expr_identifier "Math") "abs") el
+      | EJsonOpMathLog => expr_call (expr_member (expr_identifier "Math") "log2") el
+      | EJsonOpMathLog10 => expr_call (expr_member (expr_identifier "Math") "log10") el
+      | EJsonOpMathSqrt => expr_call (expr_member (expr_identifier "Math") "sqrt") el
+      | EJsonOpMathCeil => expr_call (expr_member (expr_identifier "Math") "ceil") el
+      | EJsonOpMathFloor => expr_call (expr_member (expr_identifier "Math") "floor") el
+      | EJsonOpMathTrunc => expr_call (expr_member (expr_identifier "Math") "trunc") el
       end.
 
   End Util.
@@ -136,7 +136,7 @@ Section ImpJsontoJavaScriptAst.
       | ejobject o =>
         expr_object
           (List.map
-             (fun (prop: (string * EJSON.ejson)) =>
+             (fun (prop: (string * EJson.ejson)) =>
                 let (x, v) := prop in
                 (propname_identifier x, propbody_val (ejson_to_js_ast v)))
              o)
@@ -144,49 +144,49 @@ Section ImpJsontoJavaScriptAst.
         foreign_ejson_to_ajavascript_expr fd
       end.
 
-    Fixpoint imp_json_expr_to_js_ast (exp: imp_json_expr) : expr :=
+    Fixpoint imp_ejson_expr_to_js_ast (exp: imp_ejson_expr) : expr :=
       match exp with
       | ImpExprError v => mk_expr_error
       | ImpExprVar v => expr_identifier v
       | ImpExprConst j => ejson_to_js_ast j
-      | ImpExprOp op el => imp_json_op_to_js_ast op (map imp_json_expr_to_js_ast el)
-      | ImpExprRuntimeCall rop el => mk_runtime_call rop (map imp_json_expr_to_js_ast el)
+      | ImpExprOp op el => imp_ejson_op_to_js_ast op (map imp_ejson_expr_to_js_ast el)
+      | ImpExprRuntimeCall rop el => mk_runtime_call rop (map imp_ejson_expr_to_js_ast el)
       end.
 
     Definition decl_to_js_ast (d : var * option imp_expr) :=
       match d with
       | (x, None) => (x, None)
-      | (x, Some e) => (x, Some (imp_json_expr_to_js_ast e))
+      | (x, Some e) => (x, Some (imp_ejson_expr_to_js_ast e))
       end.
 
-    Fixpoint imp_json_stmt_to_js_ast (stmt: imp_json_stmt): stat :=
+    Fixpoint imp_ejson_stmt_to_js_ast (stmt: imp_ejson_stmt): stat :=
       match stmt with
       | ImpStmtBlock decls stmts =>
         scope
-          (stat_let_decl (List.map decl_to_js_ast decls) :: (List.map imp_json_stmt_to_js_ast stmts))
+          (stat_let_decl (List.map decl_to_js_ast decls) :: (List.map imp_ejson_stmt_to_js_ast stmts))
       | ImpStmtAssign x e =>
-        stat_expr (expr_assign (expr_identifier x) None (imp_json_expr_to_js_ast e))
+        stat_expr (expr_assign (expr_identifier x) None (imp_ejson_expr_to_js_ast e))
       | ImpStmtFor x e s =>
-        stat_for_in_let nil x None (imp_json_expr_to_js_ast e)
-                        (imp_json_stmt_to_js_ast s)
+        stat_for_in_let nil x None (imp_ejson_expr_to_js_ast e)
+                        (imp_ejson_stmt_to_js_ast s)
       | ImpStmtForRange x e1 e2 s =>
         stat_for_let
           nil
-          [ (x, Some (imp_json_expr_to_js_ast e1)) ]
-          (Some (expr_binary_op (expr_identifier x) binary_op_lt (imp_json_expr_to_js_ast e2)))
+          [ (x, Some (imp_ejson_expr_to_js_ast e1)) ]
+          (Some (expr_binary_op (expr_identifier x) binary_op_lt (imp_ejson_expr_to_js_ast e2)))
           (Some (expr_unary_op unary_op_post_incr (expr_identifier x)))
-          (imp_json_stmt_to_js_ast s)
+          (imp_ejson_stmt_to_js_ast s)
       | ImpStmtIf e s1 s2 =>
         stat_if
-          (imp_json_expr_to_js_ast e)
-          (imp_json_stmt_to_js_ast s1)
-          (Some (imp_json_stmt_to_js_ast s2))
+          (imp_ejson_expr_to_js_ast e)
+          (imp_ejson_stmt_to_js_ast s1)
+          (Some (imp_ejson_stmt_to_js_ast s2))
       end.
 
-    Definition imp_json_function_to_js_ast (f: imp_function) : list string * funcbody :=
+    Definition imp_ejson_function_to_js_ast (f: imp_function) : list string * funcbody :=
       match f with
       | ImpFun v s ret =>
-        let body := imp_json_stmt_to_js_ast s in
+        let body := imp_ejson_stmt_to_js_ast s in
         let ret := scope (body :: stat_return (Some (expr_identifier ret)) :: nil) in
         let prog :=
             prog_intro strictness_true [ element_stat ret ]
@@ -194,16 +194,16 @@ Section ImpJsontoJavaScriptAst.
         ([v], funcbody_intro prog (prog_to_string prog))
       end.
 
-    Definition imp_json_to_js_ast (q: imp) : list funcdecl :=
+    Definition imp_ejson_to_js_ast (q: imp) : list funcdecl :=
       match q with
       | ImpLib l =>
         List.map
           (fun (decl: string * imp_function) =>
              let (x, f) := decl in
-             let (args, body) := imp_json_function_to_js_ast f in
+             let (args, body) := imp_ejson_function_to_js_ast f in
              funcdecl_intro x args body)
           l
       end.
   End Translation.
 
-End ImpJsontoJavaScriptAst.
+End ImpEJsontoJavaScriptAst.
